\input{settings} % add packages, settings, and declarations in settings.tex

\begin{document}

\lhead{Iliass Jabali, Ismael Aakouke} 
\rhead{MTH 1312 Spring '20 \\ Integral Calculus \\ Homework 1} 
\cfoot{\thepage\ of \pageref{LastPage}}

 \begin{enumerate}
  \textbf{Solve the homogeneous equation:
  \\\\
  a. }
  \ Putting the equation to test:
  \begin{align}
      (x^{2}+y^{2})\ \ dx-2xy\ dy \Rightarrow x^2+y^2-2xy\frac{dy}{dx}=0  \Rightarrow
      x^2+y^2-2xyy'\:=0
  \end{align}
  Using the Bernoulli equation we can find that:
  \begin{align}
      \Rightarrow  x^2+y^2-2xyy'\:=0 \ \Rightarrow 
  y'\:-\frac{1}{2x}y=\frac{x}{2}y^{-1} 
  \end{align}
  Let’s set the equation using:
  \begin{align}
      p\left(x\right)=-\frac{1}{2x}, \ \ q\left(x\right)=\frac{x}{2},\: \ \
  n=-1,  \ \ v=y^{1-n}
  \end{align}
  Dividing both sides by
  \begin{align}
      y^{-1} \ \Rightarrow 
  \frac{y'\:}{y^{-1}}-\frac{\frac{1}{2x}y}{y^{-1}}=\frac{\frac{x}{2}y^{-1}}{y^{-1}} \ \ \
  \mathrm{If\:}\nu =y^{1-n}\mathrm{\:then\:}\nu '=\left(1-n\right)\frac{y'}{y^n}.
  \end{align}
  This leaves us  with
  \begin{align}
  y'\:y-\frac{y^2}{2x}=\frac{x}{2}
  \end{align}
  Substituting 
  \begin{justify}
  y^2
  \end{justify}
   with v
  \begin{align}
  y'\:y-\frac{1}{2x}ν=\frac{x}{2}
  \end{align}
  If
  \begin{align}
  \frac{d}{dy}[v] = 2yy'
  \end{align}
  Then
  \begin{align}
  \frac{v'\:}{2}-\frac{v}{2x}=\frac{x}{2} \Rightarrow v'\:-\frac{1}{x}v=x
  \end{align}
  let’s us find a factor such as 
  \begin{center}
  z'(x) =z(x) p(x)
  \end{center}
  \begin{align}
      \frac{z'\left(x\right)}{z\left(x\right)}=\frac{z\left(x\right)p\left(x\right)}{
  z\left(x\right)} \Rightarrow \frac{
  z'\left(x\right)}{z\left(x\right)}=p\left(x\right) 
  \Rightarrow 
  \left(\ln \left(z\left(x\right)\right)\right)'\:=p\left(x\right)
  \end{align}
  This will eventually lead us to, $z\left(x\right)=\frac{e^{c_1}}{x}$
  Multiplying by the integration factor, $z(x)$ and rewriting the equation:
  \begin{align}
      v'\:-\frac{1}{x}v=x 
  \Rightarrow 
  \frac{v'\:}{x}-\frac{v}{x^2}=1
  \end{align}
  \begin{align}
      \left(\frac{1}{x}v\right)'\:=1  \Rightarrow  \ \ \frac{1}{x}v=\int 1dx \Rightarrow 
  \frac{1}{x}v=x+c_1 \quad
  \Rightarrow \quad
  v=x^2+c_1x
  \end{align}
  If we got the substitution back $v=y^2$ we are going to get: $y^2=x^2+c_1x$
  This will give us the following results:
  \begin{align}
      y=\sqrt{x^2+c_1x}\qquad and \qquad \:y=-\sqrt{x^2+c_1x}
  \end{align}
  b. 
  \begin{align}
      xydx+\left(y^2-x^2\right)dy=0 \Longrightarrow 
  xy+\left(y^2-x^2\right)\frac{dy}{dx}=0
  \Longrightarrow 
  xy+\left(y^2-x^2\right)y'\:=0 
  \end{align}
  If we isolated $y'$
  \begin{align}
      \Longrightarrow 
  y'\:=-\frac{xy}{y^2-x^2}
  \Longrightarrow 
  \ln \left(x\frac{y}{x}\right)+\frac{1}{2\left(\frac{y}{x}\right)^2}=c
  \Longrightarrow 
  \ln \left(y\right)+\frac{x^2}{2y^2}=c
  \end{align}
  c.
  \begin{align}
      \left(2x+3y\right)dx-xdy=0
  \Longrightarrow 
  2x+3y-xy'\:=0
  \end{align}
  If we replaced
  \begin{align}
      p\left(x\right)=-\frac{3}{x},\:\quad q\left(x\right)=2 
  \end{align}
  this will leave us with:
  \begin{align}
      y'\left(x\right)+p\left(x\right)\cdot y=q\left(x\right)
  \end{align}
  Finding the integration factor such as: 
  \begin{equation}
      \mu \left(x\right)\cdot p\left(x\right)=\mu '\left(x\right)
  \end{equation}
  Divide both sides by $u(x)$: 
  \begin{align}
  \frac{u'\left(x\right)}{u\left(x\right)}=\frac{u\left(x\right)p\left(x\right)}{u\left(x\right)}
  \Rightarrow \left(\ln \left(u\left(x\right)\right)\right)'\:=p\left(x\right)
  \end{align}
  this will leave us with
  \begin{align}
      \left(\ln \left(u\left(x\right)\right)\right)'\:=-\frac{3}{x}
      \Rightarrow u\left(x\right)=\frac{e^{c_1}}{x^3}
  \end{align}
  Taking off the "C" will result 
  \begin{raggedleft}
      \qquad $u\left(x\right)=\frac{1}{x^3}$
  \end{raggedleft}
  \newline
  \break
  Putting the equation  in the form 
  \begin{align}
      \left(\mu \left(x\right)\cdot \:y\left(x\right)\right)'=\mu \left(x\right)\cdot \:q\left(x\right)
  \end{align}
  Therefore, the solution to this equation is: 
  \begin{align}
      y=-x+c_1x^3
  \end{align}
  
    \newpage
\end{enumerate}

\end{document}
